Translation/SLiftSubst.v
@@ -43,6 +43,9 @@ Fixpoint lift n k t : sterm :=
   | sCongApp B1 B2 pu pA pB pv =>
     sCongApp (lift n (S k) B1) (lift n (S k) B2)
              (lift n k pu) (lift n k pA) (lift n (S k) pB) (lift n k pv)
+  | sCongSum B1 B2 pA pB =>
+    sCongSum (lift n (S k) B1) (lift n (S k) B2)
+              (lift n k pA) (lift n (S k) pB)
   | sCongEq pA pu pv => sCongEq (lift n k pA) (lift n k pu) (lift n k pv)
   | sCongRefl pA pu => sCongRefl (lift n k pA) (lift n k pu)
   | sEqToHeq p => sEqToHeq (lift n k p)
@@ -98,6 +101,9 @@ Fixpoint subst t k u :=
   | sCongApp B1 B2 pu pA pB pv =>
     sCongApp (subst t (S k) B1) (subst t (S k) B2)
              (subst t k pu) (subst t k pA) (subst t (S k) pB) (subst t k pv)
+  | sCongSum B1 B2 pA pB =>
+    sCongSum (subst t (S k) B1) (subst t (S k) B2)
+              (subst t k pA) (subst t (S k) pB)
   | sCongEq pA pu pv => sCongEq (subst t k pA) (subst t k pu) (subst t k pv)
   | sCongRefl pA pu => sCongRefl (subst t k pA) (subst t k pu)
   | sEqToHeq p => sEqToHeq (subst t k p)
@@ -167,6 +173,9 @@ Fixpoint closed_above k t :=
     closed_above (S k) B1 && closed_above (S k) B2 &&
     closed_above k pu && closed_above k pA &&
     closed_above (S k) pB && closed_above k pv
+  | sCongSum B1 B2 pA pB =>
+    closed_above (S k) B1 && closed_above (S k) B2 &&
+    closed_above k pA && closed_above (S k) pB
   | sCongEq pA pu pv =>
     closed_above k pA && closed_above k pu && closed_above k pv
   | sCongRefl pA pu => closed_above k pA && closed_above k pu
