Translation/FinalTranslation.v
@@ -102,6 +102,10 @@ Fixpoint tsl_rec (fuel : nat) (Σ : global_context) (Γ : context) (t : sterm) {
       u' <- tsl_rec fuel Σ Γ u ;;
       v' <- tsl_rec fuel Σ Γ v ;;
       myret Σ Γ (tApp u' [v'])
+    | sSum n A B =>
+      A' <- tsl_rec fuel Σ Γ A ;;
+      B' <- tsl_rec fuel Σ (Γ ,, vass n A') B ;;
+      ret (mkSum A' B')
     | sEq A u v =>
       A' <- tsl_rec fuel Σ Γ A ;;
       u' <- tsl_rec fuel Σ Γ u ;;
@@ -222,6 +226,17 @@ Fixpoint tsl_rec (fuel : nat) (Σ : global_context) (Γ : context) (t : sterm) {
       | Checked T => raise (UnexpectedTranslation "CongApp 3" pA pA' T)
       | TypeError t => raise (TypingError t)
       end
+    | sCongSum B1 B2 pA pB =>
+      pA' <- tsl_rec fuel Σ Γ pA ;;
+      match infer_hnf fuel Σ Γ pA' with
+      | Checked (tApp (tInd (mkInd "Translation.Quotes.heq" 0) _) [ _ ; A1' ; _ ; A2' ]) =>
+        pB' <- tsl_rec fuel Σ (Γ ,, vass nAnon (mkPack A1' A2')) pB ;;
+        B1' <- tsl_rec fuel Σ (Γ ,, vass nAnon A1') B1 ;;
+        B2' <- tsl_rec fuel Σ (Γ ,, vass nAnon A2') B2 ;;
+        myret Σ Γ (mkCongSum A1' A2' B1' B2' pA' pB')
+      | Checked T => raise (UnexpectedTranslation "CongSum" pA pA' T)
+      | TypeError t => raise (TypingError t)
+      end
     | sCongEq pA pu pv =>
       pA' <- tsl_rec fuel Σ Γ pA ;;
       pu' <- tsl_rec fuel Σ Γ pu ;;
@@ -310,6 +325,9 @@ Fixpoint tsl_ctx (fuel : nat) (Σ : global_context) (Γ : scontext)
 (* We define a term that mentions everything that the global context should
    have. *)
 Definition glob_term :=
+  let _ := @pp_sigT in
+  let _ := @pi1 in
+  let _ := @pi2 in
   let _ := @eq in
   let _ := @transport in
   let _ := @K in
@@ -327,6 +345,7 @@ Definition glob_term :=
   let _ := @cong_prod in
   let _ := @cong_app in
   let _ := @cong_lambda in
+  let _ := @cong_sum in
   let _ := @cong_eq in
   let _ := @cong_refl in
   let _ := @eq_to_heq in
@@ -343,65 +362,3 @@ Definition Σ : global_context :=
   pair (Datatypes.fst glob_prog) init_graph.
 
 Arguments Σ : simpl never.
-
-(* Checking for the sake of checking *)
-(* Compute (infer Σ [] tEq). *)
-(* Compute (infer Σ [] tJ). *)
-(* Compute (infer Σ [] tTransport). *)
-(* Compute (infer Σ [] tK). *)
-(* Compute (infer Σ [] tFunext). *)
-(* Compute (infer Σ [] tHeq). *)
-(* Compute (infer Σ [] tHeqToEq). *)
-(* Compute (infer Σ [] tHeqRefl). *)
-(* Compute (infer Σ [] tHeqSym). *)
-(* Compute (infer Σ [] tHeqTrans). *)
-(* Compute (infer Σ [] tHeqTransport). *)
-(* Compute (infer Σ [] tPack). *)
-(* Compute (infer Σ [] tProjT1). *)
-(* Compute (infer Σ [] tProjT2). *)
-(* Compute (infer Σ [] tProjTe). *)
-(* Compute (infer Σ [] tCongProd). *)
-(* Compute (infer Σ [] tCongLambda). *)
-(* Compute (infer Σ [] tCongApp). *)
-(* Compute (infer Σ [] tCongEq). *)
-(* Compute (infer Σ [] tCongRefl). *)
-(* Compute (infer Σ [] tEqToHeq). *)
-(* Compute (infer Σ [] tHeqTypeEq). *)
-
-(* Theorem soundness : *)
-(*   forall {Γ t A}, *)
-(*     Σ ;;; Γ |-i t : A -> *)
-(*     forall {fuel Γ' t' A'}, *)
-(*       tsl_ctx fuel Σ Γ = Success Γ' -> *)
-(*       tsl_rec fuel Σ Γ' t = Success t' -> *)
-(*       tsl_rec fuel Σ Γ' A = Success A' -> *)
-(*       Σ ;;; Γ' |-- t' : A'. *)
-(* Proof. *)
-(*   intros Γ t A h. *)
-(*   dependent induction h ; intros fuel Γ' t' A' hΓ ht hA. *)
-(*   all: destruct fuel ; try discriminate. *)
-
-(*   - cbn in ht. inversion_clear ht. *)
-(*     admit. *)
-
-(*   - cbn in ht, hA. inversion_clear ht. inversion_clear hA. *)
-(*     apply T.type_Sort. *)
-
-(*   - cbn in hA. inversion_clear hA. *)
-(*     simpl in ht. inversion ht. *)
-(*     admit. *)
-
-(*   - admit. *)
-
-(*   - admit. *)
-
-(*   - cbn in hA. inversion_clear hA. *)
-(*     cbn in ht. *)
-(*     destruct (tsl_rec fuel Σ Γ' A) ; destruct (tsl_rec fuel Σ Γ' u) ; try (now inversion ht). *)
-(*     destruct (tsl_rec fuel Σ Γ' v) ; inversion_clear ht. *)
-(*     eapply T.type_App. *)
-(*     + econstructor. econstructor. split. *)
-(*       * econstructor. *)
-(*       * cbn. f_equal. *)
-(*     + econstructor. *)
-(* Abort. *)
