Translation/ITypingInversions.v
@@ -392,6 +392,32 @@ Proof.
     all: try assumption. eapply conv_trans ; eassumption.
 Defined.
 
+Lemma inversionCongSum :
+  forall {Σ Γ B1 B2 pA pB T},
+    Σ ;;; Γ |-i sCongSum B1 B2 pA pB : T ->
+    exists s z nx ny A1 A2,
+      (Σ ;;; Γ |-i pA : sHeq (sSort s) A1 (sSort s) A2) *
+      (Σ ;;; Γ ,, (sPack A1 A2)
+       |-i pB : sHeq (sSort z) ((lift 1 1 B1){ 0 := sProjT1 (sRel 0) })
+                    (sSort z) ((lift 1 1 B2){ 0 := sProjT2 (sRel 0) })) *
+      (Σ ;;; Γ |-i A1 : sSort s) *
+      (Σ ;;; Γ |-i A2 : sSort s) *
+      (Σ ;;; Γ ,, A1 |-i B1 : sSort z) *
+      (Σ ;;; Γ ,, A2 |-i B2 : sSort z) *
+      (Σ |-i sHeq (sSort (max_sort s z)) (sSum nx A1 B1)
+                 (sSort (max_sort s z)) (sSum ny A2 B2)
+          = T).
+Proof.
+  intros Σ Γ B1 B2 pA pB T h.
+  dependent induction h.
+  - exists s, z, nx, ny, A1, A2. repeat split. all: try assumption.
+    apply conv_refl.
+  - destruct IHh1 as (s' & z & nx & ny & A1 & A2 & ?).
+    split_hyps.
+    exists s', z, nx, ny, A1, A2. repeat split. all: try assumption.
+    eapply conv_trans ; eassumption.
+Defined.
+
 Lemma inversionCongEq :
   forall {Σ Γ pA pu pv T},
     Σ ;;; Γ |-i sCongEq pA pu pv : T ->
@@ -597,6 +623,9 @@ Ltac ttinv h :=
     | sCongApp _ _ _ _ _ _ =>
       destruct (inversionCongApp h)
         as (s & z & nx & ny & A1 & A2 & u1 & u2 & v1 & v2 & hh) ;
+      splits_one hh
+    | sCongSum _ _ _ _ =>
+      destruct (inversionCongSum h) as (s & z & nx & ny & A1 & A2 & hh) ;
       splits_one hh
     | sCongEq _ _ _ =>
       destruct (inversionCongEq h) as (s & A1 & A2 & u1 & u2 & v1 & v2 & hh) ;
